Progress toward a better test compile

src/translate.hs
@@ -2,6 +2,7 @@ module Main where
 
 import qualified ConcurInterp as I
 import TranslateTest
+import ConcurCompile
 import Disk
 
 import Control.Monad (replicateM_)
@@ -24,7 +25,9 @@ main :: IO ()
 main = do
   ds <- init_disk "/dev/null"
   cs <- I.newState ds
-  t <- timeAction $ replicateM_ iterations  $ I.run cs (add_tuple_concur ((5,6),7))
-  t' <- timeAction $ replicateM_ iterations $ I.run cs (add_tuple_concur_raw ((5,6),7))
-  putStrLn $ "translate " ++ show (timePerIter t) ++ " cycles/op"
-  putStrLn $ "raw       " ++ show (timePerIter t') ++ " cycles/op"
+  t1 <- timeAction $ replicateM_ iterations  $ I.run cs (add_tuple_concur ((5,6),7) True)
+  t2 <- timeAction $ replicateM_ iterations $ I.run cs (compiled_add_tuple ((5,6),7) True)
+  t3 <- timeAction $ replicateM_ iterations  $ I.run cs (add_tuple_concur_raw ((5,6),7) True)
+  putStrLn $ "translate " ++ show (timePerIter t1) ++ " cycles/op"
+  putStrLn $ "compiled  " ++ show (timePerIter t2) ++ " cycles/op"
+  putStrLn $ "raw       " ++ show (timePerIter t3) ++ " cycles/op"
