src/TranslateTest.v
@@ -1,4 +1,4 @@
-Require Import OptimisticTranslator.
+Require Import OptimisticTranslator OptimisticCache.
 Require Prog.
 Require CCLProg.
 
@@ -18,4 +18,18 @@ Definition add_tuple (nums: nat * nat * nat) (b:bool) : prog nat :=
   }.
 
 Definition add_tuple_concur (nums: nat * nat * nat) (b:bool) :=
-  translate (add_tuple nums b) CCLProg.Locked empty_cache.
+  translate' (add_tuple nums b) CCLProg.Locked (caches empty_cache empty_cache).
+
+Import CCLProg.
+
+Definition add_tuple_concur_raw (nums: nat * nat * nat) (b:bool) : cprog _ :=
+  match b with
+  | true => 
+       n1 <- Ret (fst (fst nums));
+       n2 <- Ret (snd (fst nums));
+       n3 <- Ret (snd nums);
+       Ret (n1+n2+n3)
+  | false => 
+    _ <- CacheRead (caches empty_cache empty_cache) 0 CCLProg.Locked;
+    Ret 1
+  end.
